---
{}
---
![Teo P.7.2.2 Halvvinkelformlene](Kapittel%20X%20-%20Definisjoner%20og%20teoremer/Teo%20P.7.2.2%20Halvvinkelformlene.md)

> [!note] Argument 

Fra [P.7.6 Dobbeltvinkel-formlene](Kapittel%200%20-%20innledende%20kapittel/P.7.6%20Dobbeltvinkel-formlene.md) har vi at 
$$
\cos(2t)= \cos^2(t)-\sin^2(t) \text{ og } \sin(2t) = 2\sin (t)\cos(t).
$$
Siden $\cos^2(t)+\sin^2(t)=1$ (fra [1.](Kapittel%200%20-%20innledende%20kapittel/P.7.4%20Viktige%20identiteter.md)) får vi
$$
\begin{aligned} 
  \cos(2t) 
  & = \cos^2(t)-\sin^2(t) \\ 
  & = \cos^2(t)-\sin^2(t)+1-1 \\
  & =  \cos^2(t)-\cancel{ \sin^2(t) }+\cos^2(t)+\cancel{ \sin^2(t) }-1\\
  & = 2\cos^2(t)-1
\end{aligned} 
$$
Løser vi for $\cos^2(t)$ får vi $\displaystyle \cos^2(t) = \frac{1+\cos(2t) }{2}$.

Vi har også at $\cos^2(t) = 1-\sin^2(t) = \frac{1+\cos(2t) }{2}$. Dermed kan vi også løse for $\sin^2(t)$ og få den siste identiteten. 